Given the following loop:  
```c
*have = 0;
do {
    get = len - *have;
    if (get > max)
        get = max;
    ret = read(state->fd, buf + *have, get);
    if (ret <= 0)
        break;
    *have += (unsigned)ret;
} while (*have < len);
```
# **Proof: The Final Number of Bytes Read is \( \min(\text{len}, \text{fd\_size}) \)**  

## **Problem Statement**  

we aim to prove that upon termination:  
\[
*have_{\text{end}} = \min(\text{len}, \text{fd\_size})
\]
where `fd_size` represents the total number of bytes available in the file from the initial offset.

## **Assumption**  
We assume that **errors do not occur**, meaning that:
1. `read` **never returns a negative value**.
2. The only possible return values of `read` are:
   - A positive integer (indicating successful reading of some bytes).
   - `0` (indicating EOF has been reached).

---

## **Step 1: Establishing the Loop Invariant**  
We define the **loop invariant** as:  
\[
*have_i = \text{fd\_offset}_i - \text{fd\_offset}_0
\]
which states that **the number of bytes read equals the change in the file descriptor’s offset**.

### **Proof of the Loop Invariant**  
We prove this by induction.

1. **Base Case (\( i = 0 \))**  
   - Before the loop starts, `*have = 0` (Line 1).  
   - The initial file offset is `fd_offset_0`.  
   - Thus:
     \[
     *have_0 = \text{fd\_offset}_0 - \text{fd\_offset}_0 = 0
     \]
     The loop invariant holds.

2. **Inductive Hypothesis**  
   - Assume for some \( k \), the loop invariant holds:
     \[
     *have_k = \text{fd\_offset}_k - \text{fd\_offset}_0
     \]

3. **Inductive Step (\( i = k+1 \))**  
   - During iteration \( k+1 \), we execute:
     ```c
     *have += (unsigned)ret;   // Line 9
     ```
     which implies:
     \[
     *have_{k+1} = *have_k + \text{ret}
     \]
   - The `read` function moves the file offset forward by `ret`:
     ```c
     ret = read(state->fd, buf + *have, get);   // Line 6
     ```
     which updates the offset:
     \[
     \text{fd\_offset}_{k+1} = \text{fd\_offset}_k + \text{ret}
     \]
   - Substituting the induction hypothesis:
     \[
     *have_{k+1} = *have_k + (\text{fd\_offset}_{k+1} - \text{fd\_offset}_k)
     \]
     \[
     = (\text{fd\_offset}_k - \text{fd\_offset}_0) + (\text{fd\_offset}_{k+1} - \text{fd\_offset}_k)
     \]
     \[
     = \text{fd\_offset}_{k+1} - \text{fd\_offset}_0
     \]
   - Therefore, the loop invariant holds for all iterations.

---

## **Step 2: Proving the Exit Condition**
The loop terminates when one of the following conditions is met:

### **Case 1: EOF is reached (`ret == 0`)**  
- Since we assume no errors, `ret = 0` means we have reached **the end of the file**, meaning:
  $$
  \text{fd\_size} = \text{fd\_offset}_{\text{end}} - \text{fd\_offset}_0 
  $$
 
- From the loop invariant:
  \[
  *have_{\text{end}} = \text{fd\_offset}_{\text{end}} - \text{fd\_offset}_0 = \text{fd\_size}
  \]
  
  Since the loop condition ensures `*have ≤ len`, we get:
  \[
  *have_{\text{end}} = \min(\text{len}, \text{fd\_size})
  \]

 
### **Case 2: The loop exits because \( *\text{have} \geq \text{len} \)**  
We need to prove that:
\[
*have_{\text{end}} = \text{len}
\]
 
Since the loop condition is \( *have < \text{len} \), the loop terminates when:
\[
*have_{\text{end-1}} < \text{len}
\]
Within the loop, the calculation of `get` is as follows:
```c
get = len - *have;
if (get > max)
    get = max;
```
Thus, `get` is equal to:
\[
\min(\text{len} - *\text{have}_{\text{end-1}}, \text{max})
\]
Then, the `read` function is called:
```c
ret = read(state->fd, buf + *have, get);
```
By assumption, \( \text{ret} > 0 \), indicating that the read operation succeeded. Hence:
\[
*have_{\text{end}} = *have_{\text{end-1}} + \text{ret}
\]
 
Since `ret = get` (because `read` reads `get` bytes), we substitute:
\[
*have_{\text{end}} = *have_{\text{end-1}} + \min(\text{len} - *\text{have}_{\text{end-1}}, \text{max})
\]
It is clear that because \( *\text{have}_{\text{end-1}} < \text{len} \), `get` will never exceed \( \text{len} - *\text{have}_{\text{end-1}} \). Therefore:
\[
*have_{\text{end}} \leq \text{len}
\]
Since the loop terminates only when \( *\text{have} \geq \text{len} \), we conclude that:
\[
*have_{\text{end}} = \text{len}
\]
 
Since we assume that the `read` function always returns a positive integer (until EOF) and never signals an error, every call to `read` confirms that enough data exists in the file to meet the current read request. Successfully reading \(\text{len}\) bytes guarantees that, from the initial offset onward, there are at least \(\text{len}\) bytes available. Hence:
\[
\text{fd\_size} \ge \text{len}.
\]

Thus, we conclude that :
\[
*have_{\text{end}} = \min(\text{len}, \text{fd\_size})
\]

---

## **Step 3: Proving Loop Termination**  
To complete the proof, we show that the loop **must** terminate.

1. Since `read` **always returns a non-negative value**, the loop will exit only if:
   - `read` returns `0` (EOF), or
   - `*have` reaches `len`.
2. If `ret > 0` in every iteration, then `*have` **strictly increases**:
   \[
   *have_{k+1} > *have_k
   \]
3. Since integer `*have` is bounded by `len`, after at most `len` iterations, the loop **must** exit when `*have >= len`.
4. If `read` returns `0`, the loop exits immediately via Line 8.

Thus, **the loop is guaranteed to terminate**.

---

## **Final Conclusion**
By proving the loop invariant, the exit conditions, and the termination guarantee, we conclude:
\[
*have_{\text{end}} = \min(\text{len}, \text{fd\_size})
\]
meaning that **the total number of bytes read is the minimum of the requested `len` and the available file size (`fd_size`)**. 
